Fix formatting

rope/rope.dfy
@@ -1,3 +1,6 @@
+// This file contains an implementation of the standard rope data structure in Dafny,
+// followed by an implementation of the rope data structure used in xi-editor.
+
 module Rope {
   datatype Node = Leaf(value: string) | InternalNode(left: Rope?, right: Rope?)
 
@@ -53,10 +56,16 @@ module Rope {
         case Leaf(v) => true
         case InternalNode(left, right) =>
           (left != null ==>
-            left in this.Repr && this.Repr >= left.Repr && this !in left.Repr && left.Valid()
+            left in this.Repr &&
+            this.Repr >= left.Repr &&
+            this !in left.Repr &&
+            left.Valid()
           ) &&
           (right != null ==>
-            right in this.Repr && this.Repr >= right.Repr && this !in right.Repr && right.Valid()
+            right in this.Repr &&
+            this.Repr >= right.Repr &&
+            this !in right.Repr &&
+            right.Valid()
           )
       )
     }
@@ -87,8 +96,6 @@ module Rope {
       ensures newRope != null ==> newRope.ValidLen()
       ensures j < i ==> newRope == null
       ensures i < 0 || i >= this.Len() || j < j || j >= this.Len() ==> newRope == null
-      //ensures i == 0 && j == this.Len() - 1 && newRope != null ==> newRope.len == 0
-      // todo: len
     {
       if i < 0 || j < 0 || i >= this.Len() || j >= this.Len() || i > j
         {
@@ -316,7 +323,6 @@ module Rope {
       requires Valid()
       requires ValidLen()
       ensures i >= 0 && this.Len() > i ==> charAtIndex != ""
-      //ensures i < 0 || this.Len() <= i ==> charAtIndex == ""
       decreases Repr
     {
       match this.val
@@ -339,6 +345,252 @@ module Rope {
               { charAtIndex := left.Index(i); }
             else
               { charAtIndex := ""; }
+          }
+    }
+  }
+}
+
+
+/////////////////////////// xi-editor //////////////////////////////////////////
+
+module XiRope {
+  const MAX_CHILDREN: nat := 4
+  const MIN_CHILDREN: nat := 2
+  const MAX_LEAF_LEN: nat := 10
+  const MIN_LEAF_LEN: nat := 2   // minimum size requirement when splitting
+
+  datatype Node = Leaf(value: string) | InternalNode(children: seq<Rope>)
+
+  class Rope {
+    ghost var Repr: set<Rope>
+    ghost var Content: seq<string>
+
+    var val: Node
+    var len: int
+    var height: int
+
+    constructor Init()
+      ensures Valid()
+      ensures ValidLen()
+    {
+      val := Leaf("");
+      len := 0;
+      height := 0;
+      Repr := {this};
+      Content := [""];
+    }
+
+    constructor FromNodes(left: Rope, right: Rope)
+      requires left.ValidNonRoot() &&
+               left.ValidLen() &&
+               right.ValidNonRoot() &&
+               right.ValidLen() &&
+               left.height == right.height &&
+               left.len == left.Len() &&
+               right.len == right.Len()
+      ensures Valid()
+      ensures ValidLen()
+    {
+      Repr := left.Repr + right.Repr + {this};
+      val := InternalNode([left, right]);
+      height := left.height + 1;
+      len := left.len + right.len;
+      Content := left.Content + right.Content;
+
+    }
+
+    function method ContentLen(c: seq<string>): int
+      decreases |c|
+    {
+      if |c| == 0 then 0
+      else |c[0]| + ContentLen(c[1..])
+    }
+
+    function Len(): int
+      requires Valid()
+      reads Repr
+      decreases Repr
+    {
+      match this.val
+      case Leaf(v) => |v|
+      case InternalNode(children) => ContentLen(this.Content)
+    }
+
+    predicate ValidLen()
+      requires Valid()
+      reads this, Repr
+    {
+      match this.val
+      case Leaf(v) =>
+        this.len == |v| &&
+        ContentLen(this.Content) == |v| &&
+        |Content| == 1
+      case InternalNode(children) =>
+        this.len >= 0 && forall c: Rope :: c in children ==>
+          c.len <= this.len && c.ValidLen()
+    }
+
+    predicate ValidNonRoot()
+      reads this, Repr
+      requires MAX_LEAF_LEN >= MIN_LEAF_LEN
+      requires MIN_CHILDREN <= MAX_CHILDREN && MIN_CHILDREN >= 2
+    {
+      this in Repr &&
+      (
+        match this.val
+        case Leaf(v) => |v| <= MAX_LEAF_LEN && Content == [v] && height == 0
+        case InternalNode(children) =>
+          height >= 0 &&
+          |children| >= MIN_CHILDREN &&
+          |children| <= MAX_CHILDREN &&
+          forall c: Rope :: c in children ==>
+            c in Repr && this !in c.Repr && c.Repr < Repr && c.ValidNonRoot() &&
+            c.height == height - 1 && |c.Content| <= |Content| &&
+            forall cont: string :: cont in c.Content ==> cont in this.Content
+      )
+    }
+
+    predicate Valid()
+      reads this, Repr
+      requires MAX_LEAF_LEN >= MIN_LEAF_LEN
+      requires MIN_CHILDREN <= MAX_CHILDREN && MIN_CHILDREN >= 2
+    {
+      this in Repr &&
+      (
+        match this.val
+        case Leaf(v) => |v| <= MAX_LEAF_LEN && Content == [v] && height == 0
+        case InternalNode(children) =>
+          height >= 0 &&
+          |children| >= 2 &&
+          |children| <= MAX_CHILDREN &&
+          forall c: Rope :: c in children ==>
+            c in Repr && this !in c.Repr && c.Repr < Repr &&
+            c.ValidNonRoot() && c.height == height - 1 && |c.Content| <= |Content| &&
+            forall cont: string :: cont in c.Content ==> cont in this.Content
+      )
+    }
+
+    method Index(i: int) returns (charAtIndex: string)
+      requires Valid()
+      requires ValidLen()
+      ensures i < 0 || i >= this.len ==> charAtIndex == ""
+      decreases Repr
+    {
+      if this.len <= i || i < 0
+        { charAtIndex := ""; }
+      else
+        {
+          match this.val
+          case Leaf(v) =>
+            charAtIndex := [v[i]];
+          case InternalNode(children) =>
+            var c := 0;
+            var newI := i;
+
+            while (c + 1 < |children| && children[c].len <= newI)
+              invariant 0 <= c < |children|
+              {
+                newI := newI - children[c].len;
+                c := c + 1;
+              }
+
+            charAtIndex := children[c].Index(newI);
+        }
+    }
+
+    //method MergeNodes(rope1: Rope, rope2: Rope) returns (newRope: Rope)
+    //  requires rope1.Valid()
+    //  requires rope1.ValidLen()
+    //  requires rope2.Valid()
+    //  requires rope2.ValidLen()
+    //  ensures newRope.Valid()
+    //  ensures newRope.ValidLen()
+    //{
+    //  var children1: seq<Node> = [];
+    //  var children2: seq<Node> = []
+    //  match rope1.val
+    //  case Leaf(v) =>
+    //    children1 := [rope1.val];
+    //  case InternalNode(c) =>
+    //    children1 := c;
+    //
+    //  match rope2.val
+    //  case Leaf(v) =>
+    //    children2 := [rope2.val];
+    //  case InternalNode(c) =>
+    //    children2 := c;
+    //
+    //  if |children1| + |children2| <= MAX_CHILDREN
+    //    {
+    //      newRope := Rope.FromNodes();
+    //    }
+    //}
+
+    method Concat(rope: Rope) returns (newRope: Rope)
+      requires Valid()
+      requires ValidLen()
+      requires rope.Valid()
+      requires rope.ValidLen()
+      requires rope.height == this.height &&
+        this.len == this.Len() &&
+        rope.len == rope.Len()
+      ensures newRope.Valid()
+      ensures newRope.ValidLen()
+    {
+      // todo: implement for any input rope structure
+      newRope := new Rope.FromNodes(this, rope);
+    }
+
+    method SliceToString(i: int, j: int) returns (slice: string)
+      requires Valid()
+      requires ValidLen()
+      ensures i < 0 || i >= this.len || j >= this.len || i > j || j < 0 ==> slice == ""
+      decreases Repr
+    {
+        if i < 0 || j < 0 || i >= this.len || j >= this.len || i > j
+          {
+            slice := "";
+          }
+        else
+          {
+            match this.val
+            case Leaf(v) =>
+              slice := v[i..j];
+            case InternalNode(children) =>
+              var c := 0;
+              var newI := i;
+              var newJ := j;
+
+              while (c + 1 < |children| && children[c].len <= newI)
+              invariant 0 <= c < |children|
+              {
+                newI := newI - children[c].len;
+                newJ := newJ - children[c].len;
+                c := c + 1;
+              }
+
+              var finalSlice := "";
+
+              while (c < |children| && newJ >= 0)
+              invariant 0 <= c <= |children|
+              {
+                if newJ >= children[c].len
+                  {
+                    var s := children[c].SliceToString(newI, children[c].len - 1);
+                    finalSlice := finalSlice + s;
+                  }
+                else
+                  {
+                    var s := children[c].SliceToString(newI, newJ);
+                    finalSlice := finalSlice + s;
+                  }
+
+                newJ := newJ - children[c].len;
+                newI := 0;
+                c := c + 1;
+              }
+
+              slice := finalSlice;
           }
     }
   }
